Validator/Std/Memoize/StateRefMemoize.lean
@@ -6,41 +6,90 @@ import Validator.Std.State
 import Validator.Std.Vec
 import Validator.Std.Memoize.Memoize
 
-def MemRefT
-  {α: Type} {β: α → Type} [DecidableEq α] [Hashable α] (f: (a: α) → β a)
-  {ω} (m : Type → Type) [Monad m] [MonadLiftT (ST ω) m]
+https://github.com/leanprover/lean4/blob/1bf16f710ed7677c8331fd24f6d06ba66fc72e1c/src/Init/Control/StateRef.Lean
+https://github.com/leanprover/lean4/blob/0bcac0d46cc76fd7410e0abec06dcda33fddf4d7/src/Lean/Meta/Transform.lean#L143
+https://github.com/leanprover/lean4/blob/0bcac0d46cc76fd7410e0abec06dcda33fddf4d7/src/Lean/Util/MonadCache.lean#L62
+https://github.com/leanprover/lean4/blob/b44c7e161c13f54e8cd3da3259aa659da8f6ab70/src/Lean/Parser/Term.lean#L936
+https://github.com/leanprover/lean4/blob/b44c7e161c13f54e8cd3da3259aa659da8f6ab70/src/Lean/Elab/Frontend.lean#L27
+https://github.com/leanprover/lean4/pull/8435/files
+
+abbrev MemTableRefT'
+  {α: Type} {β: α → Type} [DecidableEq α] [Hashable α]
+  (ω) (f: (a: α) → β a) (m : Type → Type)
+  [Monad m] [MonadLiftT (ST ω) m]
   := StateRefT' ω (MemTable f) m
 
 instance
   {α: Type} {β: α → Type} [DecidableEq α] [Hashable α] (f: (a: α) → β a)
   {ω} (m : Type → Type) [Monad m] [MonadLiftT (ST ω) m]:
-  MonadStateOf (MemTable f) (StateRefT' ω (MemTable f) m) :=
+  MonadState (MemTable f) (MemTableRefT' ω f m) :=
   inferInstance
-
-def callme
-  {α: Type} [DecidableEq α] [Hashable α] {β: α -> Type}
-  (f: (a: α) -> β a)
-  [Monad m] [MonadStateOf (MemTable f) m]
-  (a: α): m { b: β a // b = f a } := do
-  let table <- MonadState.get
-  match Std.ExtDHashMap.get? table a with
-  | Option.none =>
-    let b: { b: β a // b = f a } := Subtype.mk (f a) rfl
-    MonadState.set (Std.ExtDHashMap.insert table a b)
-    return b
-  | Option.some b => return b
 
 private def MemTable.MemRefT.call
   {α: Type} [DecidableEq α] [Hashable α] {β: α -> Type} {ω} {m : Type → Type} [MonadLiftT (ST ω) m] [Monad m]
-  (f: (a: α) -> β a) (a: α): StateRefT' ω (MemTable f) m ({b: β a // b = f a}) :=
-  callme (m := StateRefT' ω (MemTable f) m) f a
+  (f: (a: α) -> β a) (a: α): MemTableRefT' ω f m ({b: β a // b = f a}) :=
+  MemTable.call (m := MemTableRefT' ω f m) f a
 
 private def MemTable.MemRefT.run
   {α: Type} [DecidableEq α] [Hashable α] {β: α -> Type} {ω} {m : Type → Type} [MonadLiftT (ST ω) m] [Monad m]
   (f: (a: α) -> β a) (a: α) (table: MemTable f): m ({b: β a // b = f a} × MemTable f) :=
-  StateRefT'.run (callme (m := StateRefT' ω (MemTable f) m) f a) table
+  StateRefT'.run (MemTable.call (m := MemTableRefT' ω f m) f a) table
 
 private def MemTable.MemRefT.run'
   {α: Type} [DecidableEq α] [Hashable α] {β: α -> Type} {ω} {m : Type → Type} [MonadLiftT (ST ω) m] [Monad m]
   (f: (a: α) -> β a) (a: α) (table: MemTable f): m ({b: β a // b = f a}) :=
-  StateRefT'.run' (callme (m := StateRefT' ω (MemTable f) m) f a) table
+  StateRefT'.run' (MemTable.call (m := MemTableRefT' ω f m) f a) table
+
+-- Example
+
+private def fib (n: Nat): Nat :=
+  match n with
+  | 0 => 0
+  | 1 => 1
+  | n + 2 => fib n + fib (n + 1)
+
+instance [Monad m] [MonadState (MemTable fib) m]: Memoize fib m where
+  call n := MemTable.call fib n
+
+private def fibM' [Monad m] [MonadState (MemTable fib) m] [Memoize fib m] (n: Nat): m { b: Nat // b = fib n } := do
+  match n with
+  | 0 => pure ⟨0, rfl⟩
+  | 1 => pure ⟨1, rfl⟩
+  | n + 2 =>
+    let fn1: { res: Nat // res = fib n } <- fibM' n
+    let fn2: { res: Nat // res = fib (n + 1) } <- fibM' (n + 1)
+    let result: { res: Nat // res = fib (n + 2) } := Subtype.mk
+      (fn1.val + fn2.val)
+      (by obtain ⟨fn1, hfn1⟩ := fn1; obtain ⟨fn2, hfn2⟩ := fn2; unfold fib; subst_vars; rfl)
+    pure result
+
+abbrev MemTableRefTIO
+  {α: Type} {β: α → Type} [DecidableEq α] [Hashable α] (f: (a: α) → β a)
+  := StateRefT (MemTable f) IO
+
+instance
+  {α: Type} {β: α → Type} [DecidableEq α] [Hashable α] (f: (a: α) → β a):
+  MonadState (MemTable f) (MemTableRefTIO f) :=
+  inferInstance
+
+instance : Memoize fib (MemTableRefTIO fib) :=
+  inferInstance
+
+#eval StateRefT'.run' (ω := IORealWorld Nat) (fibM' 4) (MemTable.init fib)
+
+def MemTableRefTIO.run'
+  (x : MemTableRefTIO fib Nat) (n: Nat) : IO { res: Nat // res = fib n } :=
+  StateRefT'.run' (fibM' n) (MemTable.init fib)
+
+private def fibM (n: Nat): IO Nat :=
+  (StateRefT'.run' (fibM' n) (MemTable.init fib))
+
+private theorem fibM'_is_correct (table: MemTable fib) (n: Nat): fib n = (StateM.run (s := table) (fibM' n)).1 := by
+  generalize (StateM.run (fibM' n) table) = x
+  obtain ⟨⟨b, hb⟩, table'⟩ := x
+  simp only
+  rw [hb]
+
+private theorem fibM_is_correct (n: Nat): fib n = fibM n := by
+  unfold fibM
+  rw [<- fibM'_is_correct]
